IrisCore/ProofRules.thy
@@ -371,6 +371,12 @@ lemma upred_existsI: "P \<turnstile> Q x \<Longrightarrow> P \<turnstile> (\<exi
 lemma upred_existsI': "(\<And>x. P x \<turnstile> Q x) \<Longrightarrow> (\<And>x. P x \<turnstile> (\<exists>\<^sub>u x. Q x))"
   by transfer' blast
 
+lemma upred_existsI_aut: "(\<And>x. Z x \<longrightarrow> (P \<turnstile> Q x)) \<Longrightarrow> (\<exists>x. Z x) \<longrightarrow> (P \<turnstile> (\<exists>\<^sub>u x. Q x))"
+  using upred_existsI by metis
+
+lemma upred_exists_lift: "\<exists>x. P \<turnstile> Q x \<Longrightarrow> P \<turnstile> (\<exists>\<^sub>u x. Q x)"
+  by transfer' auto
+
 lemma pers_forall: "(\<forall>\<^sub>u x. \<box> (P x)) \<stileturn>\<turnstile> \<box> (\<forall>\<^sub>u x. P x)"
   apply (rule upred_entail_eqI) by transfer' simp
 
