IrisCore/iPropShallow.thy
@@ -179,8 +179,10 @@ ML \<open>
 end;
 \<close>
 
+type_synonym lockG = "unit ex"
+
 setup \<open>mk_iprop [(\<^typ>\<open>graphUR auth\<close>, "graph"), (\<^typ>\<open>markingUR auth\<close>, "markings"), 
-  (\<^typ>\<open>heap_lang_proph_map\<close>, "proph")]\<close>
+  (\<^typ>\<open>heap_lang_proph_map\<close>, "proph"), (\<^typ>\<open>lockG\<close>, "lock")]\<close>
 
 lemma iprop_fp: "iProp (pre P) = P" sorry
 declare [[coercion iProp]]
